Add well-formed SSA.

mqhasm/SSA.v
@@ -112,16 +112,122 @@ Definition ssa_spec (s : spec) : SSA.spec :=
   let g := ssa_bexp m (spost s) in
   (f, p, g).
 
-Lemma upd_index_gt0 :
-  forall (m : vmap) (v : var),
-    snd (upd_index m v) > 0.
+Lemma ssa_qassign :
+  forall m1 m2 v e si,
+    ssa_instr m1 (QAssign v e) = (m2, si) ->
+    exists i,
+      (m2, i) = upd_index m1 v /\ si = SSA.QAssign (v, i) (ssa_exp m1 e).
 Proof.
-  move=> m v; rewrite /upd_index.
-  case: (VM.find v m) => /=.
-  - move=> a.
-    rewrite addn1.
+  move=> m1 m2 v e si /=.
+  set tmp := upd_index m1 v.
+  have: (tmp = upd_index m1 v) by reflexivity.
+  destruct tmp as [m2' iv].
+  move=> Hupd [Hm2' Hsi].
+  exists iv; split.
+  - rewrite Hm2'; reflexivity.
+  - symmetry; assumption.
+Qed.
+
+Lemma ssa_qsplit :
+  forall m1 m2 vh vl e p si,
+    ssa_instr m1 (QSplit vh vl e p) = (m2, si) ->
+    exists ih il m3,
+      (m3, ih) = upd_index m1 vh /\
+      (m2, il) = upd_index m3 vl /\
+      si = SSA.QSplit (vh, ih) (vl, il) (ssa_exp m1 e) p.
+Proof.
+  move=> m1 m2 vh vl e p si /=.
+  set tmp := upd_index m1 vh.
+  have: (tmp = upd_index m1 vh) by reflexivity.
+  destruct tmp as [m3 ih].
+  set tmp := upd_index m3 vl.
+  have: (tmp = upd_index m3 vl) by reflexivity.
+  destruct tmp as [m2' il].
+  move=> Hupdl Hupdh [Hm2' Hsi].
+  exists ih; exists il; exists m3; split; [idtac | split].
+  - reflexivity.
+  - rewrite -Hm2'; assumption.
+  - symmetry; assumption.
+Qed.
+
+Lemma ssa_program_empty : forall m, ssa_program m [::] = (m, [::]).
+Proof.
+  reflexivity.
+Qed.
+
+Lemma ssa_program_cons :
+  forall m1 m2 hd tl p,
+    ssa_program m1 (hd::tl) = (m2, p) ->
+    exists m3 h t,
+      ssa_instr m1 hd = (m3, h) /\ ssa_program m3 tl = (m2, t) /\ p = h::t.
+Proof.
+  move=> m1 m2 hd tl p /=.
+  set tmp := ssa_instr m1 hd.
+  have: (tmp = ssa_instr m1 hd) by reflexivity.
+  destruct tmp as [m3 h].
+  set tmp := ssa_program m3 tl.
+  have: (tmp = ssa_program m3 tl) by reflexivity.
+  destruct tmp as [m4 t].
+  move=> Htl Hhd [] Hm Hp.
+  exists m3; exists h; exists t; split; [idtac | split].
+  - reflexivity.
+  - rewrite -Htl Hm.
+    reflexivity.
+  - symmetry; exact: Hp.
+Qed.
+
+Lemma ssa_spec_unfold s :
+  exists m, SSA.spre (ssa_spec s) = ssa_bexp empty_vmap (spre s) /\
+            (m, SSA.sprog (ssa_spec s)) = ssa_program empty_vmap (sprog s) /\
+            SSA.spost (ssa_spec s) = ssa_bexp m (spost s).
+Proof.
+  destruct s as [[f p] g].
+  rewrite /ssa_spec /spre /sprog /spost /=.
+  set tmp := ssa_program empty_vmap p.
+  destruct tmp as [m sp].
+  rewrite /SSA.spre /SSA.sprog /SSA.spost /=.
+  exists m; split; [idtac | split]; reflexivity.
+Qed.
+
+Lemma upd_index_gt0 :
+  forall (m1 m2 : vmap) (v : var) (i : index),
+    (m2, i) = upd_index m1 v -> i > 0.
+Proof.
+  move=> m1 m2 v i; rewrite /upd_index.
+  case: (VM.find v m1) => /=.
+  - move=> a [] _ H.
+    rewrite addn1 in H.
+    rewrite H.
     exact: ltn0Sn.
-  - done.
+  - move=> [] _ H.
+    rewrite H.
+    done.
+Qed.
+
+Lemma upd_index_lt :
+  forall (m1 m2 : vmap) (v : var) (i : index),
+    (m2, i) = upd_index m1 v -> get_index m1 v < i.
+Proof.
+  move=> m1 m2 v i; rewrite /upd_index /get_index.
+  case: (VM.find v m1) => /=.
+  - move=> a [] _ H.
+    rewrite addn1 in H.
+    rewrite H.
+    exact: ltnSn.
+  - move=> [] _ H.
+    rewrite H.
+    done.
+Qed.
+
+Lemma upd_index_leF :
+  forall (m1 m2 : vmap) (v : var) (i : index),
+    (m2, i) = upd_index m1 v -> i <= get_index m1 v -> False.
+Proof.
+  move=> m1 m2 v i Heq Hle.
+  move: (upd_index_lt Heq) => Hlt.
+  move: (leq_ltn_trans Hle Hlt).
+  rewrite ltnn.
+  done.
 Qed.
 
 Lemma get_upd_index_eq :
@@ -165,30 +271,55 @@ Proof.
     reflexivity.
 Qed.
 
-Lemma ssa_program_empty : forall m, ssa_program m [::] = (m, [::]).
+Lemma get_upd_index_le :
+  forall (m1 m2 : vmap) (v : var) (i : index) (x : var),
+    (m2, i) = upd_index m1 v ->
+    get_index m1 x <= get_index m2 x.
 Proof.
-  reflexivity.
+  move=> m1 m2 v i x Hupd.
+  case Hxv: (x == v).
+  - rewrite (eqP Hxv).
+    rewrite (get_upd_index_eq Hupd).
+    move: (upd_index_lt Hupd) => Hlt.
+    exact: (ltnW Hlt).
+  - move/idP/negP: Hxv => Hxv.
+    rewrite (get_upd_index_neq Hxv Hupd).
+    exact: leqnn.
 Qed.
 
-Lemma ssa_program_cons :
-  forall m1 m2 hd tl p,
-    ssa_program m1 (hd::tl) = (m2, p) ->
-    exists m3 h t,
-      ssa_instr m1 hd = (m3, h) /\ ssa_program m3 tl = (m2, t) /\ p = h::t.
+Lemma ssa_instr_index_le :
+  forall m1 m2 v i si,
+    ssa_instr m1 i = (m2, si) ->
+    get_index m1 v <= get_index m2 v.
 Proof.
-  move=> m1 m2 hd tl p /=.
-  set tmp := ssa_instr m1 hd.
-  have: (tmp = ssa_instr m1 hd) by reflexivity.
-  destruct tmp as [m3 h].
-  set tmp := ssa_program m3 tl.
-  have: (tmp = ssa_program m3 tl) by reflexivity.
-  destruct tmp as [m4 t].
-  move=> Htl Hhd [] Hm Hp.
-  exists m3; exists h; exists t; split; [idtac | split].
-  - reflexivity.
-  - rewrite -Htl Hm.
-    reflexivity.
-  - symmetry; exact: Hp.
+  move=> m1 m2 v i si.
+  elim: i m1 m2 v si.
+  - move=> v e m1 m2 x si Hsi.
+    move: (ssa_qassign Hsi) => {Hsi} [i [Hupd Hsi]].
+    exact: (get_upd_index_le _ Hupd).
+  - move=> vh vl e p m1 m2 x si Hsi.
+    move: (ssa_qsplit Hsi) => {Hsi} [ih [il [m3 [Hupdh [Hupdl Hsi]]]]].
+    move: (get_upd_index_le x Hupdh) => Hle1.
+    move: (get_upd_index_le x Hupdl) => Hle2.
+    exact: (leq_trans Hle1 Hle2).
+Qed.
+
+Lemma ssa_program_index_le :
+  forall m1 m2 v p sp,
+    ssa_program m1 p = (m2, sp) ->
+    get_index m1 v <= get_index m2 v.
+Proof.
+  move=> m1 m2 v p sp.
+  elim: p m1 m2 v sp.
+  - move=> m1 m2 v sp Hsp.
+    rewrite ssa_program_empty in Hsp.
+    case: Hsp => Hm1 Hsp.
+    rewrite Hm1; exact: leqnn.
+  - move=> hd tl IH m1 m2 v sp Hsp.
+    move: (ssa_program_cons Hsp) => {Hsp} [m3 [shd [stl [Hshd [Hstl Hsp]]]]].
+    move: (ssa_instr_index_le v Hshd) => Hle1.
+    move: (IH _ _ v _ Hstl) => Hle2.
+    exact: (leq_trans Hle1 Hle2).
 Qed.
 
 Lemma ssa_eval_unop :
@@ -316,20 +447,17 @@ Lemma ssa_eval_instr :
     state_equiv m2 s2 ss2.
 Proof.
   move=> m1 m2 s1 s2 ss1 ss2 i.
-  elim: i => /=.
-  - move=> v e si.
-    set tmp := upd_index m1 v.
-    have: (tmp = upd_index m1 v) by done.
-    destruct tmp as [m' idx].
-    move=> Hupd [] Hm Hsi Heq1 Hei Hesi x.
-    rewrite Hm in Hupd => {m' Hm}.
-    rewrite -Hsi in Hesi.
+  elim: i.
+  - move=> v e si Hsi Heq /= Hei Hesi.
+    move: (ssa_qassign Hsi) => {Hsi} [idx [Hupd Hsi]].
+    move=> x.
+    rewrite Hsi in Hesi.
     inversion_clear Hei.
     inversion_clear Hesi.
     case Hxv: (x == v).
     + rewrite (State.acc_Upd_eq Hxv H0).
       rewrite (SSA.State.acc_Upd_eq _ H2).
-      * move: (ssa_eval_exp Heq1 H) => H3.
+      * move: (ssa_eval_exp Heq H) => H3.
         move: (SSA.eval_exp_unique H1 H3).
         by move/eqP=> Hn; rewrite Hn.
       * rewrite (eqP Hxv) (get_upd_index_eq Hupd).
@@ -338,19 +466,12 @@ Proof.
       rewrite (get_upd_index_neq Hxv Hupd).
       rewrite (State.acc_Upd_neq Hxv H0).
       rewrite (SSA.State.acc_Upd_neq _ H2).
-      * exact: (Heq1 x).
+      * exact: (Heq x).
       * exact: (pair_neq1 _ _ Hxv).
-  - move=> vh vl e p si.
-    set tmp := upd_index m1 vh.
-    have: (tmp = upd_index m1 vh) by done.
-    destruct tmp as [mh idh].
-    set tmp := upd_index mh vl.
-    have: (tmp = upd_index mh vl) by done.
-    destruct tmp as [ml idl].
-    move=> Hupdl Hupdh [] Hml Hsi Heq Hei Hesi.
-    rewrite Hml in Hupdl => {ml Hml}.
+  - move=> vh vl e p si Hsi Heq Hei Hesi.
+    move: (ssa_qsplit Hsi) => {Hsi} [ih [il [m3 [Hupdh [Hupdl Hsi]]]]].
     inversion_clear Hei.
-    rewrite -Hsi in Hesi; inversion_clear Hesi => {Hsi}.
+    rewrite Hsi in Hesi; inversion_clear Hesi => {Hsi}.
     move: (ssa_eval_exp_eq Heq H H3) => {H H3} Hnn4. (* n = n4 *)
     rewrite Hnn4 in H1 H2.
     rewrite -H1 in H5; rewrite -H2 in H6 => {H1 H2}. (* n0 = n1, n3 = n2 *)
@@ -359,7 +480,7 @@ Proof.
     case Hxl: (x == vl); [idtac | case Hxh: (x == vh)].
     + rewrite (State.acc_upd_eq _ _ Hxl).
       rewrite (eqP Hxl) (get_upd_index_eq Hupdl).
-      rewrite (SSA.State.acc_upd_eq _ _ (eqxx (vl, idl))).
+      rewrite (SSA.State.acc_upd_eq _ _ (eqxx (vl, il))).
       by rewrite H6.
     + move/idP/negP: Hxl => Hxl.
       rewrite (State.acc_upd_neq _ _ Hxl).
@@ -368,7 +489,7 @@ Proof.
       move: (get_upd_index_eq Hupdh) => Hidx.
       move: (get_upd_index_neq Hxl Hupdl) => Hidx'.
       rewrite -Hidx Hidx' (eqP Hxh).
-      rewrite (SSA.State.acc_upd_eq _ _ (eqxx (vh, get_index mh vh))).
+      rewrite (SSA.State.acc_upd_eq _ _ (eqxx (vh, get_index m3 vh))).
       by rewrite H5.
     + move/idP/negP: Hxl => Hxl.
       move/idP/negP: Hxh => Hxh.
@@ -391,30 +512,21 @@ Lemma ssa_eval_instr_succ :
 Proof.
   move=> m1 m2 s1 s2 ss1 i si Hi Heq Hei.
   have: (exists ss2, SSA.eval_instr ss1 si ss2).
-  - elim: i si Hi Heq Hei => /=.
-    + move=> v e si.
-      set tmp := upd_index m1 v.
-      have: (tmp = upd_index m1 v) by done.
-      destruct tmp as [m' idx].
-      move=> Hupd [] Hm Hsi Heq Hei.
+  - elim: i si Hi Heq Hei.
+    + move=> v e si Hsi Heq Hei.
+      move: (ssa_qassign Hsi) => {Hsi} [idx [Hupd Hsi]].
       inversion_clear Hei.
       pose ss2 := SSA.State.upd (v, idx) n ss1.
       exists ss2.
-      * rewrite -Hsi; apply: (SSA.EQAssign (n:=n)).
+      * rewrite Hsi; apply: (SSA.EQAssign (n:=n)).
         -- exact: (ssa_eval_exp Heq H).
         -- exact: SSA.State.Upd_upd.
-    + move=> vh vl e p si.
-      set tmp := upd_index m1 vh.
-      have: (tmp = upd_index m1 vh) by done.
-      destruct tmp as [mh idh].
-      set tmp := upd_index mh vl.
-      have: (tmp = upd_index mh vl) by done.
-      destruct tmp as [ml idl].
-      move=> Hupdl Hupdh [] Hml Hsi Heq Hei.
+    + move=> vh vl e p si Hsi Heq Hei.
+      move: (ssa_qsplit Hsi) => {Hsi} [ih [il [m3 [Hupdh [Hupdl Hsi]]]]].
       inversion_clear Hei.
-      pose ss2 := SSA.State.upd (vl, idl) n2 (SSA.State.upd (vh, idh) n1 ss1).
+      pose ss2 := SSA.State.upd (vl, il) n2 (SSA.State.upd (vh, ih) n1 ss1).
       exists ss2.
-      * rewrite -Hsi; apply: (SSA.EQSplit (n1:=n1) (n2:=n2)).
+      * rewrite Hsi; apply: (SSA.EQSplit (n1:=n1) (n2:=n2)).
         -- exact: (ssa_eval_exp Heq H).
         -- move=> x.
            reflexivity.
@@ -443,12 +555,12 @@ Proof.
     move: (SSA.eval_program_empty Hesp) => Hss.
     rewrite -Hs -Hss -Hm; exact: Heq.
   - move=> hd tl IH m1 m2 s1 s2 ss1 ss2 sp Hsp Heq Hep Hesp.
-    inversion_clear Hep.
+    move: (eval_program_cons Hep) => [s3 [Hehd Hetl]].
     move: (ssa_program_cons Hsp) => [m3 [h [t [Hh [Ht Hht]]]]].
     rewrite Hht in Hesp.
-    inversion_clear Hesp.
-    move: (ssa_eval_instr Hh Heq H H1) => Heq'.
-    exact: (IH _ _ _ _ _ _ _ Ht Heq' H0 H2).
+    move: (SSA.eval_program_cons Hesp) => [ss3 [Heshd Hestl]].
+    move: (ssa_eval_instr Hh Heq Hehd Heshd) => Heq'.
+    exact: (IH _ _ _ _ _ _ _ Ht Heq' Hetl Hestl).
 Qed.
 
 Lemma ssa_eval_program_succ :
@@ -468,10 +580,10 @@ Proof.
       exists ss1.
       rewrite -Hsp; exact: SSA.EQEmpty.
     + move=> hd tl IH m1 m2 s1 s2 ss1 sp Hsp Heq Hep.
-      inversion_clear Hep.
+      move: (eval_program_cons Hep) => [s3 [Hehd Hetl]].
       move: (ssa_program_cons Hsp) => [m3 [h [t [Hh [Ht Hht]]]]].
-      move: (ssa_eval_instr_succ Hh Heq H) => [ss3 [Heh Heqh]].
-      move: (IH m3 m2 _ _ _ t Ht Heqh H0) => [ss2 Het].
+      move: (ssa_eval_instr_succ Hh Heq Hehd) => [ss3 [Heh Heqh]].
+      move: (IH m3 m2 _ _ _ t Ht Heqh Hetl) => [ss2 Het].
       exists ss2.
       rewrite Hht; exact: (SSA.EQCons Heh Het).
   - move=> [ss2 Hesp].
@@ -538,28 +650,19 @@ Lemma dessa_eval_instr_succ :
 Proof.
   move=> m1 m2 s1 ss1 ss2 i si Hi Heq Hesi.
   have: (exists s2, eval_instr s1 i s2).
-  - elim: i si Hi Heq Hesi => /=.
-    + move=> v e si.
-      set tmp := upd_index m1 v.
-      have: (tmp = upd_index m1 v) by done.
-      destruct tmp as [m' idx].
-      move=> Hupd [] Hm Hsi Heq Hesi.
-      rewrite -Hsi in Hesi.
+  - elim: i si Hi Heq Hesi.
+    + move=> v e si Hsi Heq Hesi.
+      move: (ssa_qassign Hsi) => {Hsi} [idx [Hupd Hsi]].
+      rewrite Hsi in Hesi.
       inversion_clear Hesi.
       pose s2 := State.upd v n s1.
       exists s2.
       * apply: (EQAssign (n:=n)).
         -- exact: (dessa_eval_exp Heq H).
         -- exact: State.Upd_upd.
-    + move=> vh vl e p si.
-      set tmp := upd_index m1 vh.
-      have: (tmp = upd_index m1 vh) by done.
-      destruct tmp as [mh idh].
-      set tmp := upd_index mh vl.
-      have: (tmp = upd_index mh vl) by done.
-      destruct tmp as [ml idl].
-      move=> Hupdl Hupdh [] Hml Hsi Heq Hesi.
-      rewrite -Hsi in Hesi.
+    + move=> vh vl e p si Hsi Heq Hesi.
+      move: (ssa_qsplit Hsi) => {Hsi} [ih [il [m3 [Hupdh [Hupdl Hsi]]]]].
+      rewrite Hsi in Hesi.
       inversion_clear Hesi.
       pose s2 := State.upd vl n2 (State.upd vh n1 s1).
       exists s2.
@@ -593,9 +696,9 @@ Proof.
     + move=> hd tl IH m1 m2 s1 ss1 ss2 sp Hsp Heq Hesp.
       move: (ssa_program_cons Hsp) => [m3 [h [t [Hh [Ht Hht]]]]].
       rewrite Hht in Hesp.
-      inversion_clear Hesp.
-      move: (dessa_eval_instr_succ Hh Heq H) => [s3 [Heh Heqh]].
-      move: (IH m3 m2 _ _ _ t Ht Heqh H0) => [s4 Het].
+      move: (SSA.eval_program_cons Hesp) => [ss3 [Heshd Hestl]].
+      move: (dessa_eval_instr_succ Hh Heq Heshd) => [s3 [Heh Heqh]].
+      move: (IH m3 m2 _ _ _ t Ht Heqh Hestl) => [s4 Het].
       exists s4.
       exact: (EQCons Heh Het).
   - move=> [s2 Hep].
@@ -769,7 +872,7 @@ Proof.
   reflexivity.
 Qed.
 
-Lemma dessa_state_equiv :
+Corollary dessa_state_equiv :
   forall m s, state_equiv m (dessa_state m s) s.
 Proof.
   move=> m s x.
@@ -780,7 +883,7 @@ Qed.
 
 (** Soundness and completeness *)
 
-Lemma ssa_spec_sound (s : spec) :
+Theorem ssa_spec_sound (s : spec) :
   SSA.valid_spec (ssa_spec s) -> valid_spec s.
 Proof.
   destruct s as ((f, p), g).
@@ -798,7 +901,7 @@ Proof.
   exact: (dessa_eval_bexp Heq2 Hsg).
 Qed.
 
-Lemma ssa_spec_complete (s : spec) :
+Theorem ssa_spec_complete (s : spec) :
   valid_spec s -> SSA.valid_spec (ssa_spec s).
 Proof.
   destruct s as ((f, p), g).
@@ -814,4 +917,299 @@ Proof.
   move: (dessa_eval_bexp Heq1 Hsf) => Hf.
   move: (Hspec s1 s2 Hf Hep) => /= Hg.
   exact: (ssa_eval_bexp Heq2 Hg).
+Qed.
+
+
+
+(** Well-formed SSA *)
+
+Definition ssa_var_unchanged_instr (v : SSA.var) (i : SSA.instr) : bool :=
+  match i with
+  | SSA.QAssign v' _ => v != v'
+  | SSA.QSplit vh vl _ _ => (v != vh) && (v != vl)
+  end.
+
+Fixpoint ssa_var_unchanged_program (v : SSA.var) (p : SSA.program) : bool :=
+  match p with
+  | [::] => true
+  | hd::tl => (ssa_var_unchanged_instr v hd) && (ssa_var_unchanged_program v tl)
+  end.
+
+Fixpoint ssa_vars_unchanged_program (vs : seq SSA.var) (p : SSA.program) : bool :=
+  match vs with
+  | [::] => true
+  | hd::tl => ssa_var_unchanged_program hd p && ssa_vars_unchanged_program tl p
+  end.
+
+Fixpoint ssa_well_formed_program (p : SSA.program) : bool :=
+  match p with
+  | [::] => true
+  | hd::tl =>
+    match hd with
+    | SSA.QAssign v _ => (ssa_var_unchanged_program v tl)
+                           && (ssa_well_formed_program tl)
+    | SSA.QSplit vh vl _ _ => (ssa_var_unchanged_program vh tl)
+                                && (ssa_var_unchanged_program vl tl)
+                                && (ssa_well_formed_program tl)
+    end
+  end.
+
+Definition ssa_well_formed_spec (sp : SSA.spec) : bool :=
+  ssa_vars_unchanged_program (SSA.VS.elements (SSA.vars_bexp (SSA.spre sp)))
+                             (SSA.sprog sp)
+                             && ssa_well_formed_program (SSA.sprog sp).
+
+Lemma acc_unchanged_instr v i s1 s2 :
+  ssa_var_unchanged_instr v i ->
+  SSA.eval_instr s1 i s2 ->
+  SSA.State.acc v s2 = SSA.State.acc v s1.
+Proof.
+  elim: i.
+  - move=> v' e /= Hne Hei.
+    inversion_clear Hei.
+    rewrite (H0 v) (SSA.State.acc_upd_neq _ _ Hne).
+    reflexivity.
+  - move=> vh vl e p /= /andP [Hneh Hnel] Hei.
+    inversion_clear Hei.
+    rewrite (H0 v) (SSA.State.acc_upd_neq _ _ Hnel)
+            (SSA.State.acc_upd_neq _ _ Hneh).
+    reflexivity.
+Qed.
+
+Lemma acc_unchanged_program v p s1 s2 :
+  ssa_var_unchanged_program v p ->
+  SSA.eval_program s1 p s2 ->
+  SSA.State.acc v s2 = SSA.State.acc v s1.
+Proof.
+  elim: p s1 s2.
+  - move=> s1 s2 _ Hep.
+    rewrite (SSA.eval_program_empty Hep).
+    reflexivity.
+  - move=> hd tl IH s1 s2 /andP [Huchd Huctl] Hep.
+    move: (SSA.eval_program_cons Hep) => {Hep} [s3 [Hehd Hetl]].
+    rewrite -(acc_unchanged_instr Huchd Hehd).
+    exact: (IH _ _ Huctl Hetl).
+Qed.
+
+Lemma ssa_var_unchanged_program_cons v hd tl :
+  ssa_var_unchanged_program v (hd::tl) ->
+  ssa_var_unchanged_instr v hd /\ ssa_var_unchanged_program v tl.
+Proof.
+  move => /andP H.
+  exact: H.
+Qed.
+
+Lemma ssa_var_unchanged_program_concat v p1 p2 :
+  ssa_var_unchanged_program v (p1 ++ p2) ->
+  ssa_var_unchanged_program v p1 /\ ssa_var_unchanged_program v p2.
+Proof.
+  elim: p1 p2.
+  - move=> /= p2 H.
+    by rewrite H.
+  - move=> hd tl IH p2 /andP [Hhd Htlp2].
+    move: (IH _ Htlp2) => {IH Htlp2} [Htl Hp2].
+    by rewrite /= Hhd Htl Hp2.
+Qed.
+
+Lemma acc_unchanged_program_cons v hd tl s1 s2 s3 :
+  ssa_var_unchanged_program v (hd::tl) ->
+  SSA.eval_instr s1 hd s2 ->
+  SSA.eval_program s2 tl s3 ->
+  SSA.State.acc v s2 = SSA.State.acc v s1 /\
+  SSA.State.acc v s3 = SSA.State.acc v s1.
+Proof.
+  move=> /andP [Hunhd Huntl] Hehd Hetl.
+  move: (acc_unchanged_instr Hunhd Hehd) (acc_unchanged_program Huntl Hetl) =>
+    H21 H32.
+  rewrite H32 H21.
+  split; reflexivity.
+Qed.
+
+Lemma acc_unchanged_program_concat v p1 p2 s1 s2 s3 :
+  ssa_var_unchanged_program v (p1 ++ p2) ->
+  SSA.eval_program s1 p1 s2 ->
+  SSA.eval_program s2 p2 s3 ->
+  SSA.State.acc v s2 = SSA.State.acc v s1 /\
+  SSA.State.acc v s3 = SSA.State.acc v s1.
+Proof.
+  move=> Hun12 Hep1 Hep2.
+  move: (ssa_var_unchanged_program_concat Hun12) => {Hun12} [Hun1 Hun2].
+  rewrite (acc_unchanged_program Hun2 Hep2) (acc_unchanged_program Hun1 Hep1).
+  split; reflexivity.
+Qed.
+
+Lemma ssa_instr_le_unchanged m1 m2 i si :
+  forall v iv,
+    iv <= get_index m1 v ->
+    ssa_instr m1 i = (m2, si) ->
+    ssa_var_unchanged_instr (v, iv) si.
+Proof.
+  elim: i m1 m2 si.
+  - move=> x e m1 m2 si v iv Hiv Hsi.
+    move: (ssa_qassign Hsi) => {Hsi} [ix [Hupd Hsi]].
+    rewrite Hsi => {Hsi} /=.
+    apply/eqP => Heq; case: Heq => Hv Hi.
+    rewrite Hv Hi in Hiv => {Hv Hi}.
+    exact: (upd_index_leF Hupd Hiv).
+  - move=> vh vl e p m1 m2 si v iv Hiv Hsi.
+    move: (ssa_qsplit Hsi) => {Hsi} [ih [il [m3 [Hupdh [Hupdl Hsi]]]]].
+   rewrite Hsi => {Hsi} /=.
+    apply/andP; split; apply/eqP => Heq; case: Heq => Hv Hi.
+    + rewrite Hv Hi in Hiv => {Hv Hi v iv}.
+      exact: (upd_index_leF Hupdh Hiv).
+    + rewrite Hv Hi in Hiv => {Hv Hi v iv}.
+      move: (get_upd_index_le vl Hupdh) => Hle.
+      move: (upd_index_lt Hupdl) => Hlt.
+      move: (leq_ltn_trans Hle Hlt) => {Hle Hlt} Hlt.
+      move: (leq_ltn_trans Hiv Hlt) => {Hiv Hlt} Hlt.
+      rewrite ltnn in Hlt.
+      done.
+Qed.
+
+Lemma ssa_program_le_unchanged m1 m2 p sp :
+  forall v i,
+    i <= get_index m1 v ->
+    ssa_program m1 p = (m2, sp) ->
+    ssa_var_unchanged_program (v, i) sp.
+Proof.
+  elim: p m1 m2 sp.
+  - move=> m1 m2 sp v i Hi /= [Hm Hp].
+    by rewrite -Hp.
+  - move=> hd tl IH m1 m2 sp v i Hle Hsp.
+    move: (ssa_program_cons Hsp) => {Hsp} [m3 [shd [stl [Hshd [Hstl Hsp]]]]].
+    rewrite Hsp => {Hsp sp} /=.
+    apply/andP; split.
+    + exact: (ssa_instr_le_unchanged Hle Hshd).
+    + move: (ssa_instr_index_le v Hshd) => Hle2.
+      move: (leq_trans Hle Hle2) => {Hle Hle2} Hle.
+      exact: (IH _ _ _ _ _ Hle Hstl).
+Qed.
+
+Theorem ssa_program_well_formed m1 m2 p sp :
+  ssa_program m1 p = (m2, sp) ->
+  ssa_well_formed_program sp.
+Proof.
+  elim: p m1 m2 sp.
+  - move=> m1 m2 sp Hsp.
+    rewrite ssa_program_empty in Hsp.
+    case: Hsp => Hm Hsp.
+    rewrite -Hsp; done.
+  - move=> hd tl IH m1 m2 sp Hsp.
+    move: (ssa_program_cons Hsp) => {Hsp} [m3 [shd [stl [Hshd [Hstl Hsp]]]]].
+    rewrite Hsp => {Hsp sp}.
+    case: hd Hshd.
+    + move=> v e Hshd.
+      move: (ssa_qassign Hshd) => {Hshd} [iv [Hupd Hshd]].
+      rewrite Hshd /= => {Hshd shd}.
+      apply/andP; split.
+      * apply: (ssa_program_le_unchanged _ Hstl).
+        rewrite (get_upd_index_eq Hupd).
+        exact: leqnn.
+      * exact: (IH _ _ _ Hstl).
+    + move=> vh vl e p Hshd.
+      move: (ssa_qsplit Hshd) => {Hshd} [ih [il [m4 [Hupdh [Hupdl Hshd]]]]].
+      rewrite Hshd /= => {Hshd shd}.
+      apply/andP; split; [apply/andP; split | idtac].
+      * apply: (ssa_program_le_unchanged _ Hstl).
+        rewrite -(get_upd_index_eq Hupdh).
+        exact: (get_upd_index_le vh Hupdl).
+      * apply: (ssa_program_le_unchanged _ Hstl).
+        rewrite (get_upd_index_eq Hupdl).
+        exact: leqnn.
+      * exact: (IH _ _ _ Hstl).
+Qed.
+
+Lemma ssa_exp_var_index m e v i :
+  SSA.VS.mem (v, i) (SSA.vars_exp (ssa_exp m e)) ->
+  get_index m v = i.
+Proof.
+  elim: e m v i.
+  - move=> v m x i Hmem.
+    move/SSA.VSLemmas.memP: Hmem => Hin.
+    move: (SSA.VS.singleton_1 Hin) => /eqP [] Hv Hi.
+    rewrite -Hv; exact: Hi.
+  - move=> c m x i Hmem.
+    discriminate.
+  - move=> op e IH m x i Hmem.
+    exact: (IH _ _ _ Hmem).
+  - move=> op e1 IH1 e2 IH2 m x i Hmem.
+    move/SSA.VSLemmas.memP: Hmem => Hin.
+    move: {Hin} (SSA.VS.union_1 Hin); case => /SSA.VSLemmas.memP Hmem.
+    + apply: (IH1 _ _ _ Hmem); reflexivity.
+    + apply: (IH2 _ _ _ Hmem); reflexivity.
+Qed.
+
+Lemma ssa_bexp_var_index m e v i :
+  SSA.VS.mem (v, i) (SSA.vars_bexp (ssa_bexp m e)) ->
+  get_index m v = i.
+Proof.
+  elim: e m v i => /=.
+  - move=> m v i Hmem.
+    discriminate.
+  - move=> e1 e2 m v i Hmem.
+    rewrite SSA.VSLemmas.union_b in Hmem.
+    move/orP: Hmem; case=> Hmem;
+    apply: (ssa_exp_var_index Hmem); reflexivity.
+  - move=> e1 e2 p m v i Hmem.
+    rewrite SSA.VSLemmas.union_b in Hmem.
+    move/orP: Hmem; case=> Hmem;
+    apply: (ssa_exp_var_index Hmem); reflexivity.
+  - move=> e1 IH1 e2 IH2 m v i Hmem.
+    rewrite SSA.VSLemmas.union_b in Hmem.
+    move/orP: Hmem; case=> Hmem.
+    + apply: (IH1 _ _ _ Hmem); reflexivity.
+    + apply: (IH2 _ _ _ Hmem); reflexivity.
+Qed.
+
+Lemma ssa_spec_in_pre_unchanged s v :
+  SSA.VS.mem v (SSA.vars_bexp (SSA.spre (ssa_spec s))) ->
+  ssa_var_unchanged_program v (SSA.sprog (ssa_spec s)).
+Proof.
+  move: (ssa_spec_unfold s) => [m [Hpre [Hprog Hpost]]].
+  move=> Hmem.
+  rewrite Hpre in Hmem.
+  destruct v as [v i].
+  move: (ssa_bexp_var_index Hmem) => Hidx.
+  apply: (ssa_program_le_unchanged (m1:=empty_vmap)).
+  - by rewrite Hidx.
+  - symmetry; exact: Hprog.
+Qed.
+
+Lemma ssa_spec_unchanged_pre s :
+  ssa_vars_unchanged_program (SSA.VS.elements (SSA.vars_bexp (SSA.spre (ssa_spec s)))) (SSA.sprog (ssa_spec s)).
+Proof.
+  move: (ssa_spec_unfold s) => [m [Hpre [Hprog Hpost]]].
+  set vs := SSA.vars_bexp (SSA.spre (ssa_spec s)).
+  have: forall v : SSA.var,
+      SetoidList.InA SSA.V.eq v (SSA.VS.elements vs) -> SSA.VS.mem v vs.
+  - move=> v Hvl.
+    move: (SSA.VS.elements_2 Hvl) => Hvs.
+    apply/SSA.VSLemmas.memP.
+    assumption.
+  - set vl := SSA.VS.elements vs.
+    elim: vl.
+    + done.
+    + move=> hd tl IH H.
+      apply/andP; split.
+      * move: (H hd (SetoidList.InA_cons_hd _ (eqxx hd))) => Hmem.
+        exact: (ssa_spec_in_pre_unchanged Hmem).
+      * apply: IH => v Hin.
+        apply: H.
+        apply: SetoidList.InA_cons_tl.
+        assumption.
+Qed.
+
+Lemma ssa_spec_well_formed_program s :
+  ssa_well_formed_program (SSA.sprog (ssa_spec s)).
+Proof.
+  move: (ssa_spec_unfold s) => [m [Hpre [Hprog Hpost]]].
+  exact: (ssa_program_well_formed (Logic.eq_sym Hprog)).
+Qed.
+
+Theorem ssa_spec_well_formed s :
+  ssa_well_formed_spec (ssa_spec s).
+Proof.
+  apply/andP; split.
+  - exact: ssa_spec_unchanged_pre.
+  - exact: ssa_spec_well_formed_program.
 Qed.
