mqhasm/mQhasm.v
@@ -3,7 +3,7 @@
 
 From Coq Require Import ZArith.
 From mathcomp Require Import ssreflect ssrbool ssrnat seq eqtype.
-From Common Require Import Types Nats ZAriths Var Store.
+From Common Require Import Types Nats ZAriths FSets Var Store.
 
 Set Implicit Arguments.
 Unset Strict Implicit.
@@ -19,37 +19,56 @@ Reserved Notation "{{ f }} p {{ g }}" (at level 82).
 
 Module MakeQhasm (V : SsrOrderedType).
 
+  Module VS := FSetList.Make V.
+  Module VSLemmas := FSetLemmas VS.
+
   (** Syntax *)
 
-(*  Section Syntax.*)
+  Definition var : Type := V.t.
 
-    Definition var : Type := V.t.
+  Inductive unop : Set :=
+  | QNeg.
 
-    Inductive unop : Set :=
-    | QNeg.
+  Inductive binop : Set :=
+  | QAdd
+  | QSub
+  | QMul.
 
-    Inductive binop : Set :=
-    | QAdd
-    | QSub
-    | QMul.
+  Inductive exp : Type :=
+  | QVar : var -> exp
+  | QConst : Z -> exp
+  | QUnop : unop -> exp -> exp
+  | QBinop : binop -> exp -> exp -> exp.
 
-    Inductive exp : Type :=
-    | QVar : var -> exp
-    | QConst : Z -> exp
-    | QUnop : unop -> exp -> exp
-    | QBinop : binop -> exp -> exp -> exp.
+  Inductive instr : Type :=
+  | QAssign : var -> exp -> instr
+  | QSplit : var -> var -> exp -> positive -> instr.
 
-    Inductive instr : Type :=
-    | QAssign : var -> exp -> instr
-    | QSplit : var -> var -> exp -> positive -> instr.
+  Global Arguments QConst n%Z.
 
-    Global Arguments QConst n%Z.
+  Definition program : Type := seq instr.
 
-    Definition program : Type := seq instr.
+  Fixpoint vars_exp (e : exp) : VS.t :=
+    match e with
+    | QVar v => VS.singleton v
+    | QConst _ => VS.empty
+    | QUnop _ e => vars_exp e
+    | QBinop _ e1 e2 => VS.union (vars_exp e1) (vars_exp e2)
+    end.
 
-(*  End Syntax.*)
+  Fixpoint vars_instr (i : instr) : VS.t :=
+    match i with
+    | QAssign v e => VS.add v (vars_exp e)
+    | QSplit vh vl e _ => VS.add vh (VS.add vl (vars_exp e))
+    end.
 
-  (** Semantics *)
+  Fixpoint vars_program (p : program) : VS.t :=
+    match p with
+    | [::] => VS.empty
+    | hd::tl => VS.union (vars_instr hd) (vars_program tl)
+    end.
+
+  (** State *)
 
   Notation value := Z.
 
@@ -223,330 +242,332 @@ Module MakeQhasm (V : SsrOrderedType).
 
   End State.
 
-  Section Semantics.
+  (** Semantics *)
 
-    Definition eval_unop (op : unop) (v : value) : value :=
-      match op with
-      | QNeg => (-v)%Z
-      end.
+  Definition eval_unop (op : unop) (v : value) : value :=
+    match op with
+    | QNeg => (-v)%Z
+    end.
 
-    Definition eval_binop (op : binop) (v1 v2 : value) : value :=
-      match op with
-      | QAdd => (v1 + v2)%Z
-      | QSub => (v1 - v2)%Z
-      | QMul => (v1 * v2)%Z
-      end.
+  Definition eval_binop (op : binop) (v1 v2 : value) : value :=
+    match op with
+    | QAdd => (v1 + v2)%Z
+    | QSub => (v1 - v2)%Z
+    | QMul => (v1 * v2)%Z
+    end.
 
-    Inductive eval_exp : exp -> value -> State.t -> Prop :=
-    | EQVar :
-        forall v n s,
-          State.acc v s = Some n ->
-          eval_exp (QVar v) n s
-    | EQConst : forall n s, eval_exp (QConst n) n s
-    | EQUnop :
-        forall op e n m s,
-          eval_exp e n s ->
-          eval_unop op n = m ->
-          eval_exp (QUnop op e) m s
-    | EQBinop :
-        forall op e1 e2 v1 v2 n s,
-          eval_exp e1 v1 s ->
-          eval_exp e2 v2 s ->
-          eval_binop op v1 v2 = n ->
-          eval_exp (QBinop op e1 e2) n s.
+  Inductive eval_exp : exp -> value -> State.t -> Prop :=
+  | EQVar :
+      forall v n s,
+        State.acc v s = Some n ->
+        eval_exp (QVar v) n s
+  | EQConst : forall n s, eval_exp (QConst n) n s
+  | EQUnop :
+      forall op e n m s,
+        eval_exp e n s ->
+        eval_unop op n = m ->
+        eval_exp (QUnop op e) m s
+  | EQBinop :
+      forall op e1 e2 v1 v2 n s,
+        eval_exp e1 v1 s ->
+        eval_exp e2 v2 s ->
+        eval_binop op v1 v2 = n ->
+        eval_exp (QBinop op e1 e2) n s.
 
-    Inductive eval_instr : State.t -> instr -> State.t -> Prop :=
-    | EQAssign :
-        forall v e n s1 s2,
-          eval_exp e n s1 ->
-          State.Upd v n s1 s2 ->
-          eval_instr s1 (QAssign v e) s2
-    | EQSplit :
-        forall v1 v2 e i n1 n2 n s1 s2,
-          eval_exp e n s1 ->
-          State.Upd2 v1 n1 v2 n2 s1 s2 ->
-          n1 = fst (Z.div_eucl n (2^(Zpos i))) ->
-          n2 = snd (Z.div_eucl n (2^(Zpos i))) ->
-          eval_instr s1 (QSplit v1 v2 e i) s2.
+  Inductive eval_instr : State.t -> instr -> State.t -> Prop :=
+  | EQAssign :
+      forall v e n s1 s2,
+        eval_exp e n s1 ->
+        State.Upd v n s1 s2 ->
+        eval_instr s1 (QAssign v e) s2
+  | EQSplit :
+      forall v1 v2 e i n1 n2 n s1 s2,
+        eval_exp e n s1 ->
+        State.Upd2 v1 n1 v2 n2 s1 s2 ->
+        n1 = fst (Z.div_eucl n (2^(Zpos i))) ->
+        n2 = snd (Z.div_eucl n (2^(Zpos i))) ->
+        eval_instr s1 (QSplit v1 v2 e i) s2.
 
-    Inductive eval_program : State.t -> program -> State.t -> Prop :=
-    | EQEmpty : forall s, eval_program s nil s
-    | EQCons :
-        forall hd tl s1 s2 s3,
-          eval_instr s1 hd s2 ->
-          eval_program s2 tl s3 ->
-          eval_program s1 (hd::tl) s3.
+  Inductive eval_program : State.t -> program -> State.t -> Prop :=
+  | EQEmpty : forall s, eval_program s nil s
+  | EQCons :
+      forall hd tl s1 s2 s3,
+        eval_instr s1 hd s2 ->
+        eval_program s2 tl s3 ->
+        eval_program s1 (hd::tl) s3.
 
-    Lemma eval_qvar_unique v n m s :
-      let e := QVar v in
-      eval_exp e n s -> eval_exp e m s -> n == m.
-    Proof.
-      move=> e Hn Hm.
-      inversion_clear Hn.
-      inversion_clear Hm.
-      move: H H0; case: (State.acc v s).
-      + move=> u [] Hun [] Hum.
-        rewrite -Hun -Hum; exact: eqxx.
-      + discriminate.
-    Qed.
+  Lemma eval_qvar_unique v n m s :
+    let e := QVar v in
+    eval_exp e n s -> eval_exp e m s -> n == m.
+  Proof.
+    move=> e Hn Hm.
+    inversion_clear Hn.
+    inversion_clear Hm.
+    move: H H0; case: (State.acc v s).
+    + move=> u [] Hun [] Hum.
+      rewrite -Hun -Hum; exact: eqxx.
+    + discriminate.
+  Qed.
 
-    Lemma eval_qconst_unique v n m s :
-      let e := QConst v in
-      eval_exp e n s -> eval_exp e m s -> n == m.
-    Proof.
-      move=> e Hn Hm.
-      have: (v = n /\ v = m).
-      - split.
-        + inversion_clear Hn.
-          reflexivity.
-        + inversion_clear Hm.
-          reflexivity.
-      - move=> [] Hvn Hvm; rewrite -Hvn -Hvm; exact: eqxx.
-    Qed.
+  Lemma eval_qconst_unique v n m s :
+    let e := QConst v in
+    eval_exp e n s -> eval_exp e m s -> n == m.
+  Proof.
+    move=> e Hn Hm.
+    have: (v = n /\ v = m).
+    - split.
+      + inversion_clear Hn.
+        reflexivity.
+      + inversion_clear Hm.
+        reflexivity.
+    - move=> [] Hvn Hvm; rewrite -Hvn -Hvm; exact: eqxx.
+  Qed.
 
-    Lemma eval_qunop_unique :
-      forall (op : unop) (e : exp),
+  Lemma eval_qunop_unique :
+    forall (op : unop) (e : exp),
+      (forall (n m : value) (s : State.t),
+          eval_exp e n s -> eval_exp e m s -> n == m) ->
+      forall (n m : value) (s : State.t),
+        eval_exp (QUnop op e) n s ->
+        eval_exp (QUnop op e) m s ->
+        n == m.
+  Proof.
+    move=> op e Hind n m s Hn Hm.
+    inversion_clear Hn.
+    inversion_clear Hm.
+    move: (Hind _ _ _ H H1) => {H H1} H01.
+    rewrite -H0 -H2 (eqP H01).
+    exact: eqxx.
+  Qed.
+
+  Lemma eval_qbinop_unique :
+    forall (op : binop) (e1 : exp),
+      (forall (n m : value) (s : State.t),
+          eval_exp e1 n s -> eval_exp e1 m s -> n == m) ->
+      forall e2 : exp,
         (forall (n m : value) (s : State.t),
-            eval_exp e n s -> eval_exp e m s -> n == m) ->
+            eval_exp e2 n s -> eval_exp e2 m s -> n == m) ->
         forall (n m : value) (s : State.t),
-          eval_exp (QUnop op e) n s ->
-          eval_exp (QUnop op e) m s ->
+          eval_exp (QBinop op e1 e2) n s ->
+          eval_exp (QBinop op e1 e2) m s ->
           n == m.
-    Proof.
-      move=> op e Hind n m s Hn Hm.
-      inversion_clear Hn.
-      inversion_clear Hm.
-      move: (Hind _ _ _ H H1) => {H H1} H01.
-      rewrite -H0 -H2 (eqP H01).
-      exact: eqxx.
-    Qed.
+  Proof.
+    move=> op e1 Hind1 e2 Hind2 n m s Hn Hm.
+    inversion_clear Hn.
+    inversion_clear Hm.
+    move: (Hind1 _ _ _ H H2) => {H H2} => H10.
+    move: (Hind2 _ _ _ H0 H3) => {H0 H3} => H23.
+    rewrite -H1 -H4 (eqP H10) (eqP H23).
+    exact: eqxx.
+  Qed.
 
-    Lemma eval_qbinop_unique :
-      forall (op : binop) (e1 : exp),
-        (forall (n m : value) (s : State.t),
-            eval_exp e1 n s -> eval_exp e1 m s -> n == m) ->
-        forall e2 : exp,
-          (forall (n m : value) (s : State.t),
-              eval_exp e2 n s -> eval_exp e2 m s -> n == m) ->
-          forall (n m : value) (s : State.t),
-            eval_exp (QBinop op e1 e2) n s ->
-            eval_exp (QBinop op e1 e2) m s ->
-            n == m.
-    Proof.
-      move=> op e1 Hind1 e2 Hind2 n m s Hn Hm.
-      inversion_clear Hn.
-      inversion_clear Hm.
-      move: (Hind1 _ _ _ H H2) => {H H2} => H10.
-      move: (Hind2 _ _ _ H0 H3) => {H0 H3} => H23.
-      rewrite -H1 -H4 (eqP H10) (eqP H23).
-      exact: eqxx.
-    Qed.
+  Lemma eval_exp_unique :
+    forall e n m s, eval_exp e n s -> eval_exp e m s -> n == m.
+  Proof.
+    move=> e; elim: e.
+    - exact: eval_qvar_unique.
+    - exact: eval_qconst_unique.
+    - exact: eval_qunop_unique.
+    - exact: eval_qbinop_unique.
+  Qed.
 
-    Lemma eval_exp_unique :
-      forall e n m s, eval_exp e n s -> eval_exp e m s -> n == m.
-    Proof.
-      move=> e; elim: e.
-      - exact: eval_qvar_unique.
-      - exact: eval_qconst_unique.
-      - exact: eval_qunop_unique.
-      - exact: eval_qbinop_unique.
-    Qed.
+  Lemma eval_program_empty :
+    forall (s1 s2 : State.t),
+      eval_program s1 [::] s2 -> s1 = s2.
+  Proof.
+    move=> s1 s2 H; by inversion_clear H.
+  Qed.
 
-    Lemma eval_program_empty :
-      forall (s1 s2 : State.t),
-        eval_program s1 [::] s2 -> s1 = s2.
-    Proof.
-      move=> s1 s2 H; by inversion_clear H.
-    Qed.
+  Lemma eval_program_singleton :
+    forall (i : instr) (s1 s2 : State.t),
+      eval_program s1 ([:: i]) s2 ->
+      eval_instr s1 i s2.
+  Proof.
+    move=> i s1 s2 H; inversion_clear H.
+    move: (eval_program_empty H1) => {H1} H1.
+    rewrite -H1.
+    exact: H0.
+  Qed.
 
-    Lemma eval_program_singleton :
-      forall (i : instr) (s1 s2 : State.t),
-        eval_program s1 ([:: i]) s2 ->
-        eval_instr s1 i s2.
-    Proof.
-      move=> i s1 s2 H; inversion_clear H.
-      move: (eval_program_empty H1) => {H1} H1.
-      rewrite -H1.
-      exact: H0.
-    Qed.
+  Lemma eval_program_cons :
+    forall (hd : instr) (tl : program) (s1 s2 : State.t),
+      eval_program s1 (hd::tl) s2 ->
+      exists s3 : State.t,
+        eval_instr s1 hd s3 /\ eval_program s3 tl s2.
+  Proof.
+    move=> hd tl s1 s2 H.
+    inversion_clear H.
+    exists s3; split; assumption.
+  Qed.
 
-    Lemma eval_program_cons :
-      forall (hd : instr) (tl : program) (s1 s2 : State.t),
-        eval_program s1 (hd::tl) s2 ->
-        exists s3 : State.t,
-          eval_instr s1 hd s3 /\ eval_program s3 tl s2.
-    Proof.
-      move=> hd tl s1 s2 H.
-      inversion_clear H.
-      exists s3; split; assumption.
-    Qed.
+  Lemma eval_program_concat :
+    forall (p1 p2 : program) (s1 s2 s3 : State.t),
+      eval_program s1 p1 s2 ->
+      eval_program s2 p2 s3 ->
+      eval_program s1 (p1 ++ p2) s3.
+  Proof.
+    move=> p1; elim: p1.
+    - move=> p2 s1 s2 s3 He1 He2.
+      move: (eval_program_empty He1) => {He1} He1.
+      rewrite He1.
+      exact: He2.
+    - move=> hd tl H p2 s1 s2 s3 He1 He2.
+      move: (eval_program_cons He1) => {He1} [s4 [He1 He4]].
+      apply: (EQCons He1).
+      apply: (H _ _ _ _ He4).
+      exact: He2.
+  Qed.
 
-    Lemma eval_program_concat :
-      forall (p1 p2 : program) (s1 s2 s3 : State.t),
-        eval_program s1 p1 s2 ->
-        eval_program s2 p2 s3 ->
-        eval_program s1 (p1 ++ p2) s3.
-    Proof.
-      move=> p1; elim: p1.
-      - move=> p2 s1 s2 s3 He1 He2.
-        move: (eval_program_empty He1) => {He1} He1.
-        rewrite He1.
-        exact: He2.
-      - move=> hd tl H p2 s1 s2 s3 He1 He2.
-        move: (eval_program_cons He1) => {He1} [s4 [He1 He4]].
-        apply: (EQCons He1).
-        apply: (H _ _ _ _ He4).
-        exact: He2.
-    Qed.
-
-    Lemma eval_program_split :
-      forall (p1 p2 : program) (s1 s2 : State.t),
-        eval_program s1 (p1 ++ p2) s2 ->
-        exists s3 : State.t,
-          eval_program s1 p1 s3 /\ eval_program s3 p2 s2.
-    Proof.
-      move=> p1; elim: p1.
-      - move=> p2 s1 s2 H1.
-        exists s1; split.
-        + exact: EQEmpty.
-        + exact: H1.
-      - move=> hd tl H p2 s1 s2 He1.
-        move: (eval_program_cons He1) => {He1} [s3 [He13 He32]].
-        move: (H _ _ _ He32) => {H} [s4 [He34 He42]].
-        exists s4; split.
-        + exact: (EQCons He13 He34).
-        + exact: He42.
-    Qed.
-
-  End Semantics.
+  Lemma eval_program_split :
+    forall (p1 p2 : program) (s1 s2 : State.t),
+      eval_program s1 (p1 ++ p2) s2 ->
+      exists s3 : State.t,
+        eval_program s1 p1 s3 /\ eval_program s3 p2 s2.
+  Proof.
+    move=> p1; elim: p1.
+    - move=> p2 s1 s2 H1.
+      exists s1; split.
+      + exact: EQEmpty.
+      + exact: H1.
+    - move=> hd tl H p2 s1 s2 He1.
+      move: (eval_program_cons He1) => {He1} [s3 [He13 He32]].
+      move: (H _ _ _ He32) => {H} [s4 [He34 He42]].
+      exists s4; split.
+      + exact: (EQCons He13 He34).
+      + exact: He42.
+  Qed.
 
   (** Specification *)
 
-  Section Specification.
+  Inductive bexp : Type :=
+  | QTrue : bexp
+  | QEq : exp -> exp -> bexp
+  | QCong : exp -> exp -> positive -> bexp
+  | QAnd : bexp -> bexp -> bexp.
 
-    Inductive bexp : Type :=
-    | QTrue : bexp
-    | QEq : exp -> exp -> bexp
-    | QCong : exp -> exp -> positive -> bexp
-    | QAnd : bexp -> bexp -> bexp.
+  Fixpoint vars_bexp (e : bexp) : VS.t :=
+    match e with
+    | QTrue => VS.empty
+    | QEq e1 e2 => VS.union (vars_exp e1) (vars_exp e2)
+    | QCong e1 e2 _ => VS.union (vars_exp e1) (vars_exp e2)
+    | QAnd e1 e2 => VS.union (vars_bexp e1) (vars_bexp e2)
+    end.
 
-    Inductive eval_bexp : bexp -> bool -> State.t -> Prop :=
-    | EQTrue : forall s, eval_bexp QTrue true s
-    | EQEq :
-        forall e1 e2 n1 n2 s,
-          eval_exp e1 n1 s ->
-          eval_exp e2 n2 s ->
-          eval_bexp (QEq e1 e2) (n1 == n2) s
-    | EQCong :
-        forall e1 e2 n1 n2 p s,
-          eval_exp e1 n1 s ->
-          eval_exp e2 n2 s ->
-          eval_bexp (QCong e1 e2 p) (n1 === n2 # (Zpos p)) s
-    | EQAnd :
-        forall e1 e2 b1 b2 s,
-          eval_bexp e1 b1 s ->
-          eval_bexp e2 b2 s ->
-          eval_bexp (QAnd e1 e2) (b1 && b2) s.
+  Inductive eval_bexp : bexp -> bool -> State.t -> Prop :=
+  | EQTrue : forall s, eval_bexp QTrue true s
+  | EQEq :
+      forall e1 e2 n1 n2 s,
+        eval_exp e1 n1 s ->
+        eval_exp e2 n2 s ->
+        eval_bexp (QEq e1 e2) (n1 == n2) s
+  | EQCong :
+      forall e1 e2 n1 n2 p s,
+        eval_exp e1 n1 s ->
+        eval_exp e2 n2 s ->
+        eval_bexp (QCong e1 e2 p) (n1 === n2 # (Zpos p)) s
+  | EQAnd :
+      forall e1 e2 b1 b2 s,
+        eval_bexp e1 b1 s ->
+        eval_bexp e2 b2 s ->
+        eval_bexp (QAnd e1 e2) (b1 && b2) s.
 
-    Definition valid (f : bexp) : Prop :=
-      forall s : State.t, eval_bexp f true s.
+  Definition valid (f : bexp) : Prop :=
+    forall s : State.t, eval_bexp f true s.
 
-    Definition entails (f g : bexp) : Prop :=
-      forall s : State.t,
-        eval_bexp f true s -> eval_bexp g true s.
+  Definition entails (f g : bexp) : Prop :=
+    forall s : State.t,
+      eval_bexp f true s -> eval_bexp g true s.
 
-    Definition spec : Type := (bexp * program * bexp).
-    Definition spre (s : spec) := fst (fst s).
-    Definition sprog (s : spec) := snd (fst s).
-    Definition spost (s : spec) := snd s.
+  Definition spec : Type := (bexp * program * bexp).
+  Definition spre (s : spec) := fst (fst s).
+  Definition sprog (s : spec) := snd (fst s).
+  Definition spost (s : spec) := snd s.
 
-    Definition valid_spec (s : spec) : Prop :=
-      forall s1 s2,
-        eval_bexp (spre s) true s1 ->
-        eval_program s1 (sprog s) s2 ->
-        eval_bexp (spost s) true s2.
+  Definition valid_spec (s : spec) : Prop :=
+    forall s1 s2,
+      eval_bexp (spre s) true s1 ->
+      eval_program s1 (sprog s) s2 ->
+      eval_bexp (spost s) true s2.
 
-    Notation "{{ f }} p {{ g }}" := (valid_spec (f, p, g)) (at level 82).
+  Notation "{{ f }} p {{ g }}" := (valid_spec (f, p, g)) (at level 82).
 
-    Definition counterexample (sp : spec) (s : State.t) : Prop :=
-      eval_bexp (spre sp) true s /\
-      exists s' : State.t,
-        eval_program s (sprog sp) s' /\ eval_bexp (spost sp) false s'.
+  Definition counterexample (sp : spec) (s : State.t) : Prop :=
+    eval_bexp (spre sp) true s /\
+    exists s' : State.t,
+      eval_program s (sprog sp) s' /\ eval_bexp (spost sp) false s'.
 
-    Lemma eval_bexp_unique :
-      forall e a b s, eval_bexp e a s -> eval_bexp e b s -> a == b.
-    Proof.
-      move=> e; elim: e.
-      - move=> a b s Hea Heb.
-        inversion_clear Hea; inversion_clear Heb.
-        exact: eqxx.
-      - move=> e1 e2 a b s Hea Heb.
-        inversion_clear Hea; inversion_clear Heb.
-        rewrite (eqP (eval_exp_unique H H1)) (eqP (eval_exp_unique H0 H2)).
-        exact: eqxx.
-      - move=> e1 e2 p a b s Hea Heb.
-        inversion_clear Hea; inversion_clear Heb.
-        rewrite (eqP (eval_exp_unique H H1)) (eqP (eval_exp_unique H0 H2)).
-        exact: eqxx.
-      - move=> e1 IH1 e2 IH2 a b s Hea Heb.
-        inversion_clear Hea; inversion_clear Heb.
-        rewrite (eqP (IH1 _ _ _ H H1)) (eqP (IH2 _ _ _ H0 H2)).
-        exact: eqxx.
-    Qed.
+  Lemma eval_bexp_unique :
+    forall e a b s, eval_bexp e a s -> eval_bexp e b s -> a == b.
+  Proof.
+    move=> e; elim: e.
+    - move=> a b s Hea Heb.
+      inversion_clear Hea; inversion_clear Heb.
+      exact: eqxx.
+    - move=> e1 e2 a b s Hea Heb.
+      inversion_clear Hea; inversion_clear Heb.
+      rewrite (eqP (eval_exp_unique H H1)) (eqP (eval_exp_unique H0 H2)).
+      exact: eqxx.
+    - move=> e1 e2 p a b s Hea Heb.
+      inversion_clear Hea; inversion_clear Heb.
+      rewrite (eqP (eval_exp_unique H H1)) (eqP (eval_exp_unique H0 H2)).
+      exact: eqxx.
+    - move=> e1 IH1 e2 IH2 a b s Hea Heb.
+      inversion_clear Hea; inversion_clear Heb.
+      rewrite (eqP (IH1 _ _ _ H H1)) (eqP (IH2 _ _ _ H0 H2)).
+      exact: eqxx.
+  Qed.
 
-    Lemma spec_empty :
-      forall f g,
-        {{ f }} [::] {{ g }} -> entails f g.
-    Proof.
-      move=> f g He s Hf.
-      apply: (He s _ Hf).
-      apply: EQEmpty.
-    Qed.
+  Lemma spec_empty :
+    forall f g,
+      {{ f }} [::] {{ g }} -> entails f g.
+  Proof.
+    move=> f g He s Hf.
+    apply: (He s _ Hf).
+    apply: EQEmpty.
+  Qed.
 
-    Lemma spec_strengthing :
-      forall f g h p,
-        entails f g -> {{ g }} p {{ h }} -> {{ f }} p {{ h }}.
-    Proof.
-      move=> f g h p Hfg Hgh s1 s2 Hf Hp.
-      apply: (Hgh _ _ _ Hp).
-      exact: (Hfg _ Hf).
-    Qed.
+  Lemma spec_strengthing :
+    forall f g h p,
+      entails f g -> {{ g }} p {{ h }} -> {{ f }} p {{ h }}.
+  Proof.
+    move=> f g h p Hfg Hgh s1 s2 Hf Hp.
+    apply: (Hgh _ _ _ Hp).
+    exact: (Hfg _ Hf).
+  Qed.
 
-    Lemma spec_weakening :
-      forall f g h p,
-        {{ f }} p {{ g }} -> entails g h -> {{ f }} p {{ h }}.
-    Proof.
-      move=> f g h p Hfg Hgh s1 s2 Hf Hp.
-      apply: Hgh.
-      exact: (Hfg _ _ Hf Hp).
-    Qed.
+  Lemma spec_weakening :
+    forall f g h p,
+      {{ f }} p {{ g }} -> entails g h -> {{ f }} p {{ h }}.
+  Proof.
+    move=> f g h p Hfg Hgh s1 s2 Hf Hp.
+    apply: Hgh.
+    exact: (Hfg _ _ Hf Hp).
+  Qed.
 
-    Lemma spec_cons :
-      forall f g h hd tl,
-        {{ f }} [::hd] {{ g }} -> {{ g }} tl {{ h }} ->
-        {{ f }} (hd::tl) {{ h }}.
-    Proof.
-      move=> f g h hd tl Hhd Htl s1 s2 Hf Hp.
-      inversion_clear Hp.
-      apply: (Htl s3 _ _ H0).
-      apply: (Hhd s1 _ Hf).
-      apply: (EQCons H).
-      exact: EQEmpty.
-    Qed.
+  Lemma spec_cons :
+    forall f g h hd tl,
+      {{ f }} [::hd] {{ g }} -> {{ g }} tl {{ h }} ->
+      {{ f }} (hd::tl) {{ h }}.
+  Proof.
+    move=> f g h hd tl Hhd Htl s1 s2 Hf Hp.
+    inversion_clear Hp.
+    apply: (Htl s3 _ _ H0).
+    apply: (Hhd s1 _ Hf).
+    apply: (EQCons H).
+    exact: EQEmpty.
+  Qed.
 
-    Lemma spec_split_post :
-      forall f g1 g2 p,
-        {{ f }} p {{ g1 }} ->
-        {{ f }} p {{ g2 }} ->
-        {{ f }} p {{ QAnd g1 g2 }}.
-    Proof.
-      move=> f g1 g2 p Hg1 Hg2 s1 s2 Hf Hp.
-      move: (Hg1 s1 s2 Hf Hp) => {Hg1} Hg1.
-      move: (Hg2 s1 s2 Hf Hp) => {Hg2} Hg2.
-      exact: (EQAnd Hg1 Hg2).
-    Qed.
-
-  End Specification.
+  Lemma spec_split_post :
+    forall f g1 g2 p,
+      {{ f }} p {{ g1 }} ->
+      {{ f }} p {{ g2 }} ->
+      {{ f }} p {{ QAnd g1 g2 }}.
+  Proof.
+    move=> f g1 g2 p Hg1 Hg2 s1 s2 Hf Hp.
+    move: (Hg1 s1 s2 Hf Hp) => {Hg1} Hg1.
+    move: (Hg2 s1 s2 Hf Hp) => {Hg2} Hg2.
+    exact: (EQAnd Hg1 Hg2).
+  Qed.
 
 End MakeQhasm.
 
